Primitives.dfy
@@ -3,8 +3,8 @@ include "Common.dfy"
 
 predicate method BoolOpDenotes(op: BoolOp, b1: bool, b2: bool, result: bool) {
   match op
-    case Or  => result == b1 || b2
-    case And => result == b1 && b2
+    case Or  => result == (b1 || b2)
+    case And => result == (b1 && b2)
 }
 
 predicate method RelOpDenotes(op: RelOp, v1: int, v2: int, result: bool) {
@@ -17,9 +17,9 @@ predicate method RelOpDenotes(op: RelOp, v1: int, v2: int, result: bool) {
 
 predicate method MathOpDenotes(op: MathOp, v1: int, v2: int, result: int) {
   match op
-    case Plus      =>             result == v1 + v2
-    case Times     =>             result == v1 * v2
-    case Minus     =>             result == v1 - v2
-    case DividedBy => v2 != 0 ==> result == v1 / v2  // division by zero is undefined
-    case Mod       => v2 != 0 ==> result == v1 % v2  // division by zero is undefined
+    case Plus      =>             result == (v1 + v2)
+    case Times     =>             result == (v1 * v2)
+    case Minus     =>             result == (v1 - v2)
+    case DividedBy => v2 != 0 ==> result == (v1 / v2)  // division by zero is undefined
+    case Mod       => v2 != 0 ==> result == (v1 % v2)  // division by zero is undefined
 }
