StackSafety.dfy
@@ -1,0 +1,167 @@
+
+include "Prelude.dfy"
+include "Common.dfy"
+include "Primitives.dfy"
+include "StackSyntax.dfy"
+include "StackTyping.dfy"
+include "StackSemantics.dfy"
+
+function ArbitraryValue(t: Type): value
+  ensures TypeValue(ArbitraryValue(t)) == t
+{
+  match t
+    case Int =>
+      var v: int :| true;
+      integer(v)
+    case Bool =>
+      var v: bool :| true;
+      boolean(v)
+    case Unit =>
+      unit
+}
+
+lemma ProgressBool(o: BoolOp, v1: bool, v2: bool)
+  ensures exists v :: BoolOpDenotes(o, v1, v2, v)
+{
+  match o
+    case And => assert BoolOpDenotes(o, v1, v2, v1 && v2);
+    case Or  => assert BoolOpDenotes(o, v1, v2, v1 || v2);
+}
+
+lemma ProgressRel(o: RelOp, v1: int, v2: int)
+  ensures exists v :: RelOpDenotes(o, v1, v2, v)
+{
+  match o
+    case Eq  => assert RelOpDenotes(o, v1, v2, v1 == v2);
+    case NEq => assert RelOpDenotes(o, v1, v2, v1 != v2);
+    case LT  => assert RelOpDenotes(o, v1, v2, v1 <  v2);
+    case LTE => assert RelOpDenotes(o, v1, v2, v1 <= v2);
+}
+
+lemma ProgressMath(o: MathOp, v1: int, v2: int)
+  ensures exists v :: MathOpDenotes(o, v1, v2, v)
+{
+  match o
+    case Plus => assert MathOpDenotes(o, v1, v2, v1 + v2);
+    case Times => assert MathOpDenotes(o, v1, v2, v1 * v2);
+    case Minus => assert MathOpDenotes(o, v1, v2, v1 - v2);
+    case DividedBy =>
+      if v2 != 0 {
+        assert MathOpDenotes(o, v1, v2, v1 / v2);
+      } else {
+        var v :| true;
+        assert MathOpDenotes(o, v1, v2, v);
+      }
+    case Mod =>
+      if v2 != 0 {
+        assert MathOpDenotes(o, v1, v2, v1 % v2);
+      } else {
+        var v :| true;
+        assert MathOpDenotes(o, v1, v2, v);
+      }
+}
+
+lemma ProgressOperation(o: operation, s: sigma)
+  requires exists t: Type :: TypeOperation(o) == (TypeSigma(s), t)
+  ensures exists v :: StepOperation(o, s, v) && TypeValue(v) == TypeOperation(o).1
+{
+  match o
+    case not =>
+      assert StepOperation(o, s, boolean(!s[0].getBoolean));
+    case const(x) =>
+      assert StepOperation(o, s, x);
+    case read(t) =>
+      assert StepOperation(o, s, ArbitraryValue(t));
+    case printf(format) =>
+      assert StepOperation(o, s, unit);
+    case binary(o) =>
+      match o
+        case MathOp(o) =>
+          ProgressMath(o, s[0].getInteger, s[1].getInteger);
+          var v :| MathOpDenotes(o, s[0].getInteger, s[1].getInteger, v);
+          assert StepOperation(binary(MathOp(o)), s, integer(v));
+        case BoolOp(o) =>
+          ProgressBool(o, s[0].getBoolean, s[1].getBoolean);
+          var v :| BoolOpDenotes(o, s[0].getBoolean, s[1].getBoolean, v);
+          assert StepOperation(binary(BoolOp(o)), s, boolean(v));
+        case RelOp(o) =>
+          ProgressRel(o, s[0].getInteger, s[1].getInteger);
+          var v :| RelOpDenotes(o, s[0].getInteger, s[1].getInteger, v);
+          assert StepOperation(binary(RelOp(o)), s, boolean(v));
+}
+
+lemma ProgressCommand(c: command, s: sigma, S: Sigma)
+  requires Prefix(S, TypeSigma(s))
+  requires exists S' :: TypeCommand(c, S) == Just(S')
+  ensures  exists s' :: StepCommand(c, s, s')
+                  //&& Prefix(TypeCommand(c, S).FromJust, TypeSigma(s'))
+{
+  match c
+    case pop(n) =>
+      assert StepCommand(c, s, s[n..]);
+    case load(n) =>
+      assert StepCommand(c, s, [s[n]] + s);
+    case store(n) =>
+      assert StepCommand(c, s, s[n := s[0]][1..]);
+    case apply(n, o) =>
+      var (So, t) := TypeOperation(o);
+      assert TypeSigma(s[..n]) == So;
+      ProgressOperation(o, s[..n]);
+      var v :| StepOperation(o, s[..n], v);
+      assert StepCommand(c, s, [v] + s[n..]);
+}
+
+lemma ProgressJump(SigmaH: Sigma, D: Delta, d: delta, j: jump, Phi: Phi, phi: phi)
+  requires TypeProgram(SigmaH, D, d)
+  requires TypeJump(D, SigmaH, j, Phi)
+  requires ValidStack(D, phi)
+  requires SubPhi(Phi, TypePhi(D, phi))
+  requires j != halt
+  ensures  exists phi', b' :: StepJump(d, j, phi, phi', b')
+                        //&& TypeBlock(D, SigmaH, b', TypePhi(D, phi'))
+{
+  match j
+    case goto(nu) =>
+      assert StepJump(d, j, phi, phi, d[nu]);
+    case branch(nu1, nu2) =>
+      var nu := phi[0].0;
+      var s  := phi[0].1;
+      var b  := s[0].getBoolean;
+      assert StepJump(d, j, phi, [(nu, s[1..])] + phi[1..], d[if b then nu1 else nu2]);
+    case call(n, nuJ, nuR) =>
+      var nu := phi[0].0;
+      var s  := phi[0].1;
+      var (s1, s2) := Split(n, s);
+      assert StepJump(d, j, phi, [(nuR, s1), (nu, s2)] + phi[1..], d[nuJ]);
+    case ret(n) =>
+      var nuR := phi[0].0;
+      var s_check := phi[0].1[..n];
+      var nu := phi[1].0;
+      var s  := phi[1].1;
+      assert StepJump(d, j, phi, [(nu, s_check + s)] + phi[2..], d[nuR]);
+}
+
+lemma ProgressBlock(SigmaH: Sigma, D: Delta, d: delta, b: block, Phi: Phi, phi: phi)
+  requires TypeProgram(SigmaH, D, d)
+  requires TypeBlock(D, SigmaH, b, Phi)
+  requires ValidStack(D, phi)
+  requires SubPhi(Phi, TypePhi(D, phi))
+  ensures  (b == (Nil, halt) && Prefix(SigmaH, Phi.out[0].1)) ||
+           exists phi', b' :: StepBlock(d, b, phi, phi', b')
+{
+  var (cs, j) := b;
+  match cs
+    case Cons(c, cs) =>
+      var nu := phi[0].0;
+      var s := phi[0].1;
+      var S := Phi.out[0].1;
+      ProgressCommand(c, s, S);
+      var s' :| StepCommand(c, s, s');
+      assert StepBlock(d, b, phi, phi[0 := (nu, s')], (cs, j));
+    case Nil =>
+      if j != halt {
+        ProgressJump(SigmaH, D, d, j, Phi, phi);
+        var phi', b' :| StepJump(d, j, phi, phi', b');
+        assert StepBlock(d, b, phi, phi', b');
+      }
+}
